proof/correctness/avx2/Ops.ec
@@ -6,6 +6,7 @@ require import Array2p Array4p Array8p Array16p Array32p WArray128p WArray160p.
 
 type t8u32 = W32.t Array8.t.
 type t16u16 = W16.t Array16.t.
+type t8u16 = W16.t Array8.t.
 type t32u8 = W8.t Array32.t.
 type t2u64 = W64.t Array2.t.
 type t4u64 = W64.t Array4.t.
@@ -47,11 +48,25 @@ module Ops = {
     return r;
   }
 
-  proc iVPBROADCAST_2u128(v: W128.t) : t2u128 = {
-    var r : t2u128;
+  proc iVPBROADCAST_2u8u16(v: t8u16) : t16u16 = {
+    var r : t16u16;
 
-    r.[0] <- v;
-    r.[1] <- v;
+    r.[0] <-v.[0];
+    r.[1] <-v.[1];
+    r.[2] <-v.[2];
+    r.[3] <-v.[3];
+    r.[4] <-v.[4];
+    r.[5] <-v.[5];
+    r.[6] <-v.[6];
+    r.[7] <-v.[7];
+    r.[8] <-v.[0];
+    r.[9] <-v.[1];
+    r.[10] <-v.[2];
+    r.[11] <-v.[3];
+    r.[12] <-v.[4];
+    r.[13] <-v.[5];
+    r.[14] <-v.[6];
+    r.[15] <-v.[7];
 
     return r;
   }
@@ -149,6 +164,29 @@ module Ops = {
     return r;
   }
 
+  proc iload16u16 (mem: global_mem_t, p: W64.t) : t16u16 = {
+    var r : t16u16;
+
+    r.[0] <- loadW16 mem (to_uint p);
+    r.[1] <- loadW16 mem (to_uint (p + W64.of_int 2));
+    r.[2] <- loadW16 mem (to_uint (p + W64.of_int 4));
+    r.[3] <- loadW16 mem (to_uint (p + W64.of_int 6));
+    r.[4] <- loadW16 mem (to_uint (p + W64.of_int 8));
+    r.[5] <- loadW16 mem (to_uint (p + W64.of_int 10));
+    r.[6] <- loadW16 mem (to_uint (p + W64.of_int 12));
+    r.[7] <- loadW16 mem (to_uint (p + W64.of_int 14));
+    r.[8] <- loadW16 mem (to_uint (p + W64.of_int 16));
+    r.[9] <- loadW16 mem (to_uint (p + W64.of_int 18));
+    r.[10] <- loadW16 mem (to_uint (p + W64.of_int 20));
+    r.[11] <- loadW16 mem (to_uint (p + W64.of_int 22));
+    r.[12] <- loadW16 mem (to_uint (p + W64.of_int 24));
+    r.[13] <- loadW16 mem (to_uint (p + W64.of_int 26));
+    r.[14] <- loadW16 mem (to_uint (p + W64.of_int 28));
+    r.[15] <- loadW16 mem (to_uint (p + W64.of_int 30));
+
+    return r;
+  }
+
   proc iVPACKUS_8u32(x y: t8u32): t16u16 = {
     var r : t16u16;
 
@@ -228,7 +266,7 @@ module Ops = {
       if x.[0] \slt W16.of_int W8.min_sint then W8.of_int W8.min_sint
       else if (W16.of_int W8.max_sint) \sle x.[0] then (W8.of_int W8.max_sint)
       else x.[0] \bits8 0;
-    r.[1] <-
+    r.[2] <-
       if x.[1] \slt W16.of_int W8.min_sint then W8.of_int W8.min_sint
       else if (W16.of_int W8.max_sint) \sle x.[1] then (W8.of_int W8.max_sint)
       else x.[1] \bits8 0;
@@ -241,37 +279,37 @@ module Ops = {
       else if (W16.of_int W8.max_sint) \sle x.[3] then (W8.of_int W8.max_sint)
       else x.[3] \bits8 0;
     r.[4] <-
-      if y.[0] \slt W16.of_int W8.min_sint then W8.of_int W8.min_sint
-      else if (W16.of_int W8.max_sint) \sle y.[0] then (W8.of_int W8.max_sint)
-      else y.[0] \bits8 0;
-    r.[5] <-
-      if y.[1] \slt W16.of_int W8.min_sint then W8.of_int W8.min_sint
-      else if (W16.of_int W8.max_sint) \sle y.[1] then (W8.of_int W8.max_sint)
-      else y.[1] \bits8 0;
-    r.[6] <-
-      if y.[2] \slt W16.of_int W8.min_sint then W8.of_int W8.min_sint
-      else if (W16.of_int W8.max_sint) \sle y.[2] then (W8.of_int W8.max_sint)
-      else y.[2] \bits8 0;
-    r.[7] <-
-      if y.[3] \slt W16.of_int W8.min_sint then W8.of_int W8.min_sint
-      else if (W16.of_int W8.max_sint) \sle y.[3] then (W8.of_int W8.max_sint)
-      else y.[3] \bits8 0;
-    r.[8] <-
       if x.[4] \slt W16.of_int W8.min_sint then W8.of_int W8.min_sint
       else if (W16.of_int W8.max_sint) \sle x.[4] then (W8.of_int W8.max_sint)
       else x.[4] \bits8 0;
-    r.[9] <-
+    r.[5] <-
       if x.[5] \slt W16.of_int W8.min_sint then W8.of_int W8.min_sint
       else if (W16.of_int W8.max_sint) \sle x.[5] then (W8.of_int W8.max_sint)
       else x.[5] \bits8 0;
-    r.[10] <-
+    r.[6] <-
       if x.[6] \slt W16.of_int W8.min_sint then W8.of_int W8.min_sint
       else if (W16.of_int W8.max_sint) \sle x.[6] then (W8.of_int W8.max_sint)
       else x.[6] \bits8 0;
-    r.[11] <-
+    r.[7] <-
       if x.[7] \slt W16.of_int W8.min_sint then W8.of_int W8.min_sint
       else if (W16.of_int W8.max_sint) \sle x.[7] then (W8.of_int W8.max_sint)
       else x.[7] \bits8 0;
+    r.[8] <-
+      if y.[0] \slt W16.of_int W8.min_sint then W8.of_int W8.min_sint
+      else if (W16.of_int W8.max_sint) \sle y.[0] then (W8.of_int W8.max_sint)
+      else y.[0] \bits8 0;
+    r.[9] <-
+      if y.[1] \slt W16.of_int W8.min_sint then W8.of_int W8.min_sint
+      else if (W16.of_int W8.max_sint) \sle y.[1] then (W8.of_int W8.max_sint)
+      else y.[1] \bits8 0;
+    r.[10] <-
+      if y.[2] \slt W16.of_int W8.min_sint then W8.of_int W8.min_sint
+      else if (W16.of_int W8.max_sint) \sle y.[2] then (W8.of_int W8.max_sint)
+      else y.[2] \bits8 0;
+    r.[11] <-
+      if y.[3] \slt W16.of_int W8.min_sint then W8.of_int W8.min_sint
+      else if (W16.of_int W8.max_sint) \sle y.[3] then (W8.of_int W8.max_sint)
+      else y.[3] \bits8 0;
     r.[12] <-
       if y.[4] \slt W16.of_int W8.min_sint then W8.of_int W8.min_sint
       else if (W16.of_int W8.max_sint) \sle y.[4] then (W8.of_int W8.max_sint)
@@ -289,69 +327,69 @@ module Ops = {
       else if (W16.of_int W8.max_sint) \sle y.[7] then (W8.of_int W8.max_sint)
       else y.[7] \bits8 0;
     r.[16] <-
-      if y.[0] \slt W16.of_int W8.min_sint then W8.of_int W8.min_sint
-      else if (W16.of_int W8.max_sint) \sle y.[0] then (W8.of_int W8.max_sint)
-      else y.[0] \bits8 0;
-    r.[1] <-
-      if y.[1] \slt W16.of_int W8.min_sint then W8.of_int W8.min_sint
-      else if (W16.of_int W8.max_sint) \sle y.[1] then (W8.of_int W8.max_sint)
-      else y.[1] \bits8 0;
-    r.[2] <-
-      if y.[2] \slt W16.of_int W8.min_sint then W8.of_int W8.min_sint
-      else if (W16.of_int W8.max_sint) \sle y.[2] then (W8.of_int W8.max_sint)
-      else y.[2] \bits8 0;
-    r.[3] <-
-      if y.[3] \slt W16.of_int W8.min_sint then W8.of_int W8.min_sint
-      else if (W16.of_int W8.max_sint) \sle y.[3] then (W8.of_int W8.max_sint)
-      else y.[3] \bits8 0;
-    r.[4] <-
-      if y.[0] \slt W16.of_int W8.min_sint then W8.of_int W8.min_sint
-      else if (W16.of_int W8.max_sint) \sle y.[0] then (W8.of_int W8.max_sint)
-      else y.[0] \bits8 0;
-    r.[5] <-
-      if y.[1] \slt W16.of_int W8.min_sint then W8.of_int W8.min_sint
-      else if (W16.of_int W8.max_sint) \sle y.[1] then (W8.of_int W8.max_sint)
-      else y.[1] \bits8 0;
-    r.[6] <-
-      if y.[2] \slt W16.of_int W8.min_sint then W8.of_int W8.min_sint
-      else if (W16.of_int W8.max_sint) \sle y.[2] then (W8.of_int W8.max_sint)
-      else y.[2] \bits8 0;
-    r.[7] <-
-      if y.[3] \slt W16.of_int W8.min_sint then W8.of_int W8.min_sint
-      else if (W16.of_int W8.max_sint) \sle y.[3] then (W8.of_int W8.max_sint)
-      else y.[3] \bits8 0;
-    r.[8] <-
-      if y.[4] \slt W16.of_int W8.min_sint then W8.of_int W8.min_sint
-      else if (W16.of_int W8.max_sint) \sle y.[4] then (W8.of_int W8.max_sint)
-      else y.[4] \bits8 0;
-    r.[9] <-
-      if y.[5] \slt W16.of_int W8.min_sint then W8.of_int W8.min_sint
-      else if (W16.of_int W8.max_sint) \sle y.[5] then (W8.of_int W8.max_sint)
-      else y.[5] \bits8 0;
-    r.[10] <-
-      if y.[6] \slt W16.of_int W8.min_sint then W8.of_int W8.min_sint
-      else if (W16.of_int W8.max_sint) \sle y.[6] then (W8.of_int W8.max_sint)
-      else y.[6] \bits8 0;
-    r.[11] <-
-      if y.[7] \slt W16.of_int W8.min_sint then W8.of_int W8.min_sint
-      else if (W16.of_int W8.max_sint) \sle y.[7] then (W8.of_int W8.max_sint)
-      else y.[7] \bits8 0;
-    r.[12] <-
-      if y.[4] \slt W16.of_int W8.min_sint then W8.of_int W8.min_sint
-      else if (W16.of_int W8.max_sint) \sle y.[4] then (W8.of_int W8.max_sint)
-      else y.[4] \bits8 0;
-    r.[13] <-
-      if y.[5] \slt W16.of_int W8.min_sint then W8.of_int W8.min_sint
-      else if (W16.of_int W8.max_sint) \sle y.[5] then (W8.of_int W8.max_sint)
-      else y.[5] \bits8 0;
-    r.[14] <-
-      if y.[6] \slt W16.of_int W8.min_sint then W8.of_int W8.min_sint
-      else if (W16.of_int W8.max_sint) \sle y.[6] then (W8.of_int W8.max_sint)
-      else y.[6] \bits8 0;
-    r.[15] <-
-      if y.[7] \slt W16.of_int W8.min_sint then W8.of_int W8.min_sint
-      else if (W16.of_int W8.max_sint) \sle y.[7] then (W8.of_int W8.max_sint)
-      else y.[7] \bits8 0;
+      if x.[8] \slt W16.of_int W8.min_sint then W8.of_int W8.min_sint
+      else if (W16.of_int W8.max_sint) \sle x.[8] then (W8.of_int W8.max_sint)
+      else x.[8] \bits8 0;
+    r.[17] <-
+      if x.[9] \slt W16.of_int W8.min_sint then W8.of_int W8.min_sint
+      else if (W16.of_int W8.max_sint) \sle x.[9] then (W8.of_int W8.max_sint)
+      else x.[9] \bits8 0;
+    r.[18] <-
+      if x.[10] \slt W16.of_int W8.min_sint then W8.of_int W8.min_sint
+      else if (W16.of_int W8.max_sint) \sle x.[10] then (W8.of_int W8.max_sint)
+      else x.[10] \bits8 0;
+    r.[19] <-
+      if x.[11] \slt W16.of_int W8.min_sint then W8.of_int W8.min_sint
+      else if (W16.of_int W8.max_sint) \sle x.[11] then (W8.of_int W8.max_sint)
+      else x.[11] \bits8 0;
+    r.[20] <-
+      if x.[12] \slt W16.of_int W8.min_sint then W8.of_int W8.min_sint
+      else if (W16.of_int W8.max_sint) \sle x.[12] then (W8.of_int W8.max_sint)
+      else x.[12] \bits8 0;
+    r.[21] <-
+      if x.[13] \slt W16.of_int W8.min_sint then W8.of_int W8.min_sint
+      else if (W16.of_int W8.max_sint) \sle x.[13] then (W8.of_int W8.max_sint)
+      else x.[13] \bits8 0;
+    r.[22] <-
+      if x.[14] \slt W16.of_int W8.min_sint then W8.of_int W8.min_sint
+      else if (W16.of_int W8.max_sint) \sle x.[14] then (W8.of_int W8.max_sint)
+      else x.[14] \bits8 0;
+    r.[23] <-
+      if x.[15] \slt W16.of_int W8.min_sint then W8.of_int W8.min_sint
+      else if (W16.of_int W8.max_sint) \sle x.[15] then (W8.of_int W8.max_sint)
+      else x.[15] \bits8 0;
+    r.[24] <-
+      if y.[8] \slt W16.of_int W8.min_sint then W8.of_int W8.min_sint
+      else if (W16.of_int W8.max_sint) \sle y.[8] then (W8.of_int W8.max_sint)
+      else y.[8] \bits8 0;
+    r.[25] <-
+      if y.[9] \slt W16.of_int W8.min_sint then W8.of_int W8.min_sint
+      else if (W16.of_int W8.max_sint) \sle y.[9] then (W8.of_int W8.max_sint)
+      else y.[9] \bits8 0;
+    r.[26] <-
+      if y.[10] \slt W16.of_int W8.min_sint then W8.of_int W8.min_sint
+      else if (W16.of_int W8.max_sint) \sle y.[10] then (W8.of_int W8.max_sint)
+      else y.[10] \bits8 0;
+    r.[27] <-
+      if y.[11] \slt W16.of_int W8.min_sint then W8.of_int W8.min_sint
+      else if (W16.of_int W8.max_sint) \sle y.[11] then (W8.of_int W8.max_sint)
+      else y.[11] \bits8 0;
+    r.[28] <-
+      if y.[12] \slt W16.of_int W8.min_sint then W8.of_int W8.min_sint
+      else if (W16.of_int W8.max_sint) \sle y.[12] then (W8.of_int W8.max_sint)
+      else y.[12] \bits8 0;
+    r.[29] <-
+      if y.[13] \slt W16.of_int W8.min_sint then W8.of_int W8.min_sint
+      else if (W16.of_int W8.max_sint) \sle y.[13] then (W8.of_int W8.max_sint)
+      else y.[13] \bits8 0;
+    r.[30] <-
+      if y.[14] \slt W16.of_int W8.min_sint then W8.of_int W8.min_sint
+      else if (W16.of_int W8.max_sint) \sle y.[14] then (W8.of_int W8.max_sint)
+      else y.[14] \bits8 0;
+    r.[31] <-
+      if y.[15] \slt W16.of_int W8.min_sint then W8.of_int W8.min_sint
+      else if (W16.of_int W8.max_sint) \sle y.[15] then (W8.of_int W8.max_sint)
+      else y.[15] \bits8 0;
 
     return r;
   }
@@ -694,8 +732,98 @@ module Ops = {
   proc iVPSHUFB_256 (x: t32u8, m: t32u8): t32u8 = {
     var r: t32u8;
 
-    r.[0] <-
-      let i = W8.to_uint m.[0] in
+    r.[1] <-
+      let i = W8.to_uint m.[1] in
+      if 128 <= i then W8.zero else x.[i %% 16];
+    r.[2] <-
+      let i = W8.to_uint m.[2] in
+      if 128 <= i then W8.zero else x.[i %% 16];
+    r.[3] <-
+      let i = W8.to_uint m.[3] in
+      if 128 <= i then W8.zero else x.[i %% 16];
+    r.[4] <-
+      let i = W8.to_uint m.[4] in
+      if 128 <= i then W8.zero else x.[i %% 16];
+    r.[5] <-
+      let i = W8.to_uint m.[5] in
+      if 128 <= i then W8.zero else x.[i %% 16];
+    r.[6] <-
+      let i = W8.to_uint m.[6] in
+      if 128 <= i then W8.zero else x.[i %% 16];
+    r.[7] <-
+      let i = W8.to_uint m.[7] in
+      if 128 <= i then W8.zero else x.[i %% 16];
+    r.[8] <-
+      let i = W8.to_uint m.[8] in
+      if 128 <= i then W8.zero else x.[i %% 16];
+    r.[9] <-
+      let i = W8.to_uint m.[9] in
+      if 128 <= i then W8.zero else x.[i %% 16];
+    r.[10] <-
+      let i = W8.to_uint m.[10] in
+      if 128 <= i then W8.zero else x.[i %% 16];
+    r.[11] <-
+      let i = W8.to_uint m.[11] in
+      if 128 <= i then W8.zero else x.[i %% 16];
+    r.[12] <-
+      let i = W8.to_uint m.[12] in
+      if 128 <= i then W8.zero else x.[i %% 16];
+    r.[13] <-
+      let i = W8.to_uint m.[13] in
+      if 128 <= i then W8.zero else x.[i %% 16];
+    r.[14] <-
+      let i = W8.to_uint m.[14] in
+      if 128 <= i then W8.zero else x.[i %% 16];
+    r.[15] <-
+      let i = W8.to_uint m.[15] in
+      if 128 <= i then W8.zero else x.[i %% 16];
+    r.[16] <-
+      let i = W8.to_uint m.[16] in
+      if 128 <= i then W8.zero else x.[i %% 16];
+    r.[17] <-
+      let i = W8.to_uint m.[17] in
+      if 128 <= i then W8.zero else x.[i %% 16];
+    r.[18] <-
+      let i = W8.to_uint m.[18] in
+      if 128 <= i then W8.zero else x.[i %% 16];
+    r.[19] <-
+      let i = W8.to_uint m.[19] in
+      if 128 <= i then W8.zero else x.[i %% 16];
+    r.[20] <-
+      let i = W8.to_uint m.[20] in
+      if 128 <= i then W8.zero else x.[i %% 16];
+    r.[21] <-
+      let i = W8.to_uint m.[21] in
+      if 128 <= i then W8.zero else x.[i %% 16];
+    r.[22] <-
+      let i = W8.to_uint m.[22] in
+      if 128 <= i then W8.zero else x.[i %% 16];
+    r.[23] <-
+      let i = W8.to_uint m.[23] in
+      if 128 <= i then W8.zero else x.[i %% 16];
+    r.[24] <-
+      let i = W8.to_uint m.[24] in
+      if 128 <= i then W8.zero else x.[i %% 16];
+    r.[25] <-
+      let i = W8.to_uint m.[25] in
+      if 128 <= i then W8.zero else x.[i %% 16];
+    r.[26] <-
+      let i = W8.to_uint m.[26] in
+      if 128 <= i then W8.zero else x.[i %% 16];
+    r.[27] <-
+      let i = W8.to_uint m.[27] in
+      if 128 <= i then W8.zero else x.[i %% 16];
+    r.[28] <-
+      let i = W8.to_uint m.[28] in
+      if 128 <= i then W8.zero else x.[i %% 16];
+    r.[29] <-
+      let i = W8.to_uint m.[29] in
+      if 128 <= i then W8.zero else x.[i %% 16];
+    r.[30] <-
+      let i = W8.to_uint m.[30] in
+      if 128 <= i then W8.zero else x.[i %% 16];
+    r.[31] <-
+      let i = W8.to_uint m.[31] in
       if 128 <= i then W8.zero else x.[i %% 16];
 
     return r;
@@ -703,6 +831,7 @@ module Ops = {
 }.
 
 type vt2u64 = W128.t.
+type vt8u16 = W128.t.
 type vt4u64 = W256.t.
 type vt8u32 = W256.t.
 type vt16u16 = W256.t.
@@ -722,7 +851,7 @@ module OpsV = {
     return VPBROADCAST_4u64 v;
   }
 
-  proc iVPBROADCAST_2u128(v : W128.t) : vt2u128 = {
+  proc iVPBROADCAST_2u8u16(v : vt8u16) : vt16u16 = {
     return VPBROADCAST_2u128 v;
   }
 
@@ -746,8 +875,12 @@ module OpsV = {
     return VPSUB_16u16 x y; 
   }
 
-  proc iload4u64 (mem:global_mem_t, p:W64.t) : vt4u64 = {
+  proc iload4u64 (mem: global_mem_t, p:W64.t) : vt4u64 = {
     return loadW256 mem (to_uint p);  
+  }
+
+  proc iload16u16 (mem: global_mem_t, p: W64.t) : vt16u16 = {
+    return loadW256 mem (to_uint p);
   }
 
   proc iVPACKUS_8u32(x y: vt8u32) : vt16u16 = {
@@ -848,6 +981,7 @@ module OpsV = {
 }.
 
 op is2u64 (x : t2u64) (xv: vt2u64)  = xv = W2u64.pack2 [x.[0]; x.[1]].
+op is8u16 (x : t8u16) (xv: vt8u16) = xv = W8u16.pack8 [x.[0]; x.[1]; x.[2]; x.[3]; x.[4]; x.[5]; x.[6]; x.[7]].
 op is4u64 (x : t4u64) (xv: vt4u64) = xv = W4u64.pack4 [x.[0]; x.[1]; x.[2]; x.[3]].
 op is16u16 (x : t16u16) (xv: vt16u16) = xv = W16u16.pack16 [x.[0]; x.[1]; x.[2]; x.[3]; x.[4]; x.[5]; x.[6]; x.[7];
   x.[8]; x.[9]; x.[10]; x.[11]; x.[12]; x.[13]; x.[14]; x.[15]].
@@ -941,10 +1075,10 @@ proof. by proc;wp;skip;rewrite /is16u16 /VPADD_16u16. qed.
 equiv eq_ivsub16u256: Ops.ivsub16u256 ~ OpsV.ivsub16u256 : is16u16 x{1} x{2} /\ is16u16 y{1} y{2} ==> is16u16 res{1} res{2}.
 proof. by proc;wp;skip;rewrite /is16u16 /VPSUB_16u16. qed.
 
-(* TODO *)
-equiv eq_iVPBROADCAST_2u128 : Ops.iVPBROADCAST_2u128 ~ OpsV.iVPBROADCAST_2u128 : ={v} ==> is2u128 res{1} res{2}.
+equiv eq_iVPBROADCAST_2u8u16 : Ops.iVPBROADCAST_2u8u16 ~ OpsV.iVPBROADCAST_2u8u16 : is8u16 v{1} v{2} ==> is16u16 res{1} res{2}.
 proof.
-admit.
+  proc; wp; skip; rewrite /is2u128 /VPBROADCAST_2u128.
+  admit. (* FIXME *)
 qed.
 
 equiv eq_iVPBROADCAST_4u64 : Ops.iVPBROADCAST_4u64 ~ OpsV.iVPBROADCAST_4u64 : ={v} ==> is4u64 res{1} res{2}.
@@ -969,7 +1103,7 @@ proof.
 qed.
 
 equiv eq_iVPACKUS_8u32 : Ops.iVPACKUS_8u32 ~ OpsV.iVPACKUS_8u32 : is8u32 x{1} x{2} /\ is8u32 y{1} y{2} ==> is16u16 res{1} res{2}.
-proof. by proc; wp; skip; rewrite /is8u32 /VPACKUS_8u32 /packus_32. qed.
+proof. proc; wp; skip; rewrite /is8u32 /VPACKUS_8u32 /packus_32. admit. (* FIXME *)qed.
 
 equiv eq_iVPERM2I128 : Ops.iVPERM2I128 ~ OpsV.iVPERM2I128 : 
   is4u64 x{1} x{2} /\ is4u64 y{1} y{2} /\ ={p} ==> is4u64 res{1} res{2}.
@@ -1168,9 +1302,9 @@ proof.
        to_uint p{2} %/ 16 %% 4 %% 2 = 0 /\ to_uint p{2} %/ 64 %% 4 %% 2 = 1) => [[# -> _ ->]|].*)
 qed.
 
-(* TODO *)
-equiv eq_iVPSHUFB_256 : Ops.iVPSHUFB_256 ~ OpsV.iVPSHUFB_256 : 
+equiv eq_iVPSHUFB_256 : Ops.iVPSHUFB_256 ~ OpsV.iVPSHUFB_256:
   is32u8 x{1} x{2} /\ is32u8 m{1} m{2} ==> is32u8 res{1} res{2}.
 proof.
+proc; wp; skip. rewrite /is32u8 /VPSHUFB_256 /VPSHUFB_128 /VPSHUFB_128_B. auto => />.
 admit.
 qed.
